theories/GenericTyping.v
@@ -168,11 +168,11 @@ Section RedDefinitions.
       isWfPair Γ A B (tPair A' B' a b)
   | NeWfPair : forall n : term, [Γ |- n ~ n : tSig A B] -> isWfPair Γ A B n.
 
-  Record EvalStep Γ t u k v := {
-    evstep_eval : ∑ k', murec (eval true (tApp (erase t) (qNat u))) k' = Some (k, qNat v);
-    evstep_nil : (forall k', k' < k -> [ Γ |- qRun t u k' ≅ tZero : tNat ]);
-    evstep_val : [ Γ |- qRun t u k ≅ tSucc (qNat v) : tNat ];
-  }.
+(*   Record EvalStep Γ t u k v := { *)
+(*     evstep_eval : ∑ k', murec (eval true (tApp (erase t) (qNat u))) k' = Some (k, qNat v); *)
+(*     evstep_nil : (forall k', k' < k -> [ Γ |- qRun t u k' ≅ tZero : tNat ]); *)
+(*     evstep_val : [ Γ |- qRun t u k ≅ tSucc (qNat v) : tNat ]; *)
+(*   }. *)
 
 End RedDefinitions.
 
@@ -340,19 +340,19 @@ Section GenericTyping.
       [Γ |- y : A] ->
       [Γ |- e : tId A x y] ->
       [Γ |- tIdElim A x P hr y e : P[e .: y..]];
-    ty_quote {Γ} {t} :
-      [ Γ |- t ≅ t : arr tNat tNat ] ->
-      [ Γ |- tQuote t : tNat ];
-    ty_step {Γ} {t u} :
-      [ Γ |- t ≅ t : arr tNat tNat ] ->
-      [ Γ |- u ≅ u : tNat ] ->
-      [ Γ |- run : arr tNat (arr tNat tPNat) ] ->
-      [ Γ |- tStep t u : tNat ];
-    ty_reflect {Γ} {t t' u u'} :
-      [ Γ |- t ≅ t' : arr tNat tNat ] ->
-      [ Γ |- u ≅ u' : tNat ] ->
-      [ Γ |- run : arr tNat (arr tNat tPNat) ] ->
-      [ Γ |- tReflect t u : tTotal t' u' ];
+(*     ty_quote {Γ} {t} : *)
+(*       [ Γ |- t ≅ t : arr tNat tNat ] -> *)
+(*       [ Γ |- tQuote t : tNat ]; *)
+(*     ty_step {Γ} {t u} : *)
+(*       [ Γ |- t ≅ t : arr tNat tNat ] -> *)
+(*       [ Γ |- u ≅ u : tNat ] -> *)
+(*       [ Γ |- run : arr tNat (arr tNat tPNat) ] -> *)
+(*       [ Γ |- tStep t u : tNat ]; *)
+(*     ty_reflect {Γ} {t t' u u'} : *)
+(*       [ Γ |- t ≅ t' : arr tNat tNat ] -> *)
+(*       [ Γ |- u ≅ u' : tNat ] -> *)
+(*       [ Γ |- run : arr tNat (arr tNat tPNat) ] -> *)
+(*       [ Γ |- tReflect t u : tTotal t' u' ]; *)
     ty_exp {Γ t A A'} : [Γ |- t : A'] -> [Γ |- A ⤳* A'] -> [Γ |- t : A] ;
     ty_conv {Γ t A A'} : [Γ |- t : A'] -> [Γ |- A' ≅ A] -> [Γ |- t : A] ;
   }.
@@ -490,29 +490,29 @@ Section GenericTyping.
       [Γ |- y ≅ y' : A] ->
       [Γ |- e ~ e' : tId A x y] ->
       [Γ |- tIdElim A x P hr y e ~ tIdElim A' x' P' hr' y' e' : P[e .: y..]];
-    convneu_quote {Γ n n'} :
-        [Γ |- n ≅ n' : arr tNat tNat] ->
-        dnf n -> dnf n' ->
-        ~ closed0 n -> ~ closed0 n' ->
-        [Γ |- tQuote n ~ tQuote n' : tNat];
-    convneu_step {Γ t t' t₀ u u' u₀} :
-      [Γ |- t ≅ t' : arr tNat tNat] ->
-      [Γ |- u ≅ u' : tNat] ->
-      [Γ |- t ≅ t₀ : arr tNat tNat] ->
-      [Γ |- u ≅ u₀ : tNat] ->
-      [Γ |- run : arr tNat (arr tNat tPNat)] ->
-      dnf t -> dnf t' -> dnf u -> dnf u' ->
-      (~ is_closedn 0 t) + (~ is_closedn 0 u) -> (~ is_closedn 0 t') + (~ is_closedn 0 u') ->
-      [Γ |- tStep t u ~ tStep t' u' : tNat];
-    convneu_reflect {Γ t t' t₀ u u' u₀} :
-      [Γ |- t ≅ t' : arr tNat tNat] ->
-      [Γ |- u ≅ u' : tNat] ->
-      [Γ |- t ≅ t₀ : arr tNat tNat] ->
-      [Γ |- u ≅ u₀ : tNat] ->
-      [Γ |- run : arr tNat (arr tNat tPNat)] ->
-      dnf t -> dnf t' -> dnf u -> dnf u' ->
-      (~ is_closedn 0 t) + (~ is_closedn 0 u) -> (~ is_closedn 0 t') + (~ is_closedn 0 u') ->
-      [Γ |- tReflect t u ~ tReflect t' u' : tTotal t₀ u₀];
+(*     convneu_quote {Γ n n'} : *)
+(*         [Γ |- n ≅ n' : arr tNat tNat] -> *)
+(*         dnf n -> dnf n' -> *)
+(*         ~ closed0 n -> ~ closed0 n' -> *)
+(*         [Γ |- tQuote n ~ tQuote n' : tNat]; *)
+(*     convneu_step {Γ t t' t₀ u u' u₀} : *)
+(*       [Γ |- t ≅ t' : arr tNat tNat] -> *)
+(*       [Γ |- u ≅ u' : tNat] -> *)
+(*       [Γ |- t ≅ t₀ : arr tNat tNat] -> *)
+(*       [Γ |- u ≅ u₀ : tNat] -> *)
+(*       [Γ |- run : arr tNat (arr tNat tPNat)] -> *)
+(*       dnf t -> dnf t' -> dnf u -> dnf u' -> *)
+(*       (~ is_closedn 0 t) + (~ is_closedn 0 u) -> (~ is_closedn 0 t') + (~ is_closedn 0 u') -> *)
+(*       [Γ |- tStep t u ~ tStep t' u' : tNat]; *)
+(*     convneu_reflect {Γ t t' t₀ u u' u₀} : *)
+(*       [Γ |- t ≅ t' : arr tNat tNat] -> *)
+(*       [Γ |- u ≅ u' : tNat] -> *)
+(*       [Γ |- t ≅ t₀ : arr tNat tNat] -> *)
+(*       [Γ |- u ≅ u₀ : tNat] -> *)
+(*       [Γ |- run : arr tNat (arr tNat tPNat)] -> *)
+(*       dnf t -> dnf t' -> dnf u -> dnf u' -> *)
+(*       (~ is_closedn 0 t) + (~ is_closedn 0 u) -> (~ is_closedn 0 t') + (~ is_closedn 0 u') -> *)
+(*       [Γ |- tReflect t u ~ tReflect t' u' : tTotal t₀ u₀]; *)
   }.
 
   Class RedTypeProperties :=
@@ -604,41 +604,41 @@ Section GenericTyping.
       [Γ |- y : A] ->
       [Γ |- e ⤳* e' : tId A x y] ->
       [Γ |- tIdElim A x P hr y e ⤳* tIdElim A x P hr y e' : P[e .: y..]];
-    redtm_evalquote {Γ t} :
-      [Γ |- t ≅ t : arr tNat tNat] -> dnf t -> closed0 t ->
-      [Γ |- tQuote t ⤳* qNat (quote (erase t)) : tNat];
-    redtm_quote {Γ t t'} :
-      [Γ |- t ≅ t' : arr tNat tNat] ->
-      [ t ⇶* t' ] ->
-      [Γ |- tQuote t ⤳* tQuote t' : tNat ];
-    redtm_evalstep {Γ t u k n} :
-      [Γ |- t ≅ t : arr tNat tNat] ->
-      [Γ |- run : arr tNat (arr tNat tPNat)] ->
-      dnf t -> closed0 t ->
-      EvalStep Γ t u k n ->
-      [Γ |- tStep t (qNat u) ⤳* qNat k : tNat ];
-    redtm_step {Γ t t' u u'} :
-      [Γ |- t ≅ t' : arr tNat tNat] ->
-      [Γ |- u ≅ u' : tNat] ->
-      [Γ |- run : arr tNat (arr tNat tPNat)] ->
-      [ t ⇶* t' ] ->
-      [ u ⇶* u' ] ->
-      dnf t' -> dnf u' ->
-      [Γ |- tStep t u ⤳* tStep t' u' : tNat ];
-    redtm_evalreflect {Γ t t₀ u k n} :
-      [Γ |- t ≅ t₀ : arr tNat tNat] ->
-      [Γ |- run : arr tNat (arr tNat tPNat)] ->
-      dnf t₀ -> closed0 t₀ ->
-      EvalStep Γ t₀ u k n ->
-      [Γ |- tReflect t₀ (qNat u) ⤳* qEvalTm k n : tTotal t (qNat u) ];
-    redtm_reflect {Γ t t' u u'} :
-      [Γ |- t ≅ t' : arr tNat tNat] ->
-      [Γ |- u ≅ u' : tNat] ->
-      [Γ |- run : arr tNat (arr tNat tPNat)] ->
-      [ t ⇶* t' ] ->
-      [ u ⇶* u' ] ->
-      dnf t' -> dnf u' ->
-      [Γ |- tReflect t u ⤳* tReflect t' u' : tTotal t u ];
+(*     redtm_evalquote {Γ t} : *)
+(*       [Γ |- t ≅ t : arr tNat tNat] -> dnf t -> closed0 t -> *)
+(*       [Γ |- tQuote t ⤳* qNat (quote (erase t)) : tNat]; *)
+(*     redtm_quote {Γ t t'} : *)
+(*       [Γ |- t ≅ t' : arr tNat tNat] -> *)
+(*       [ t ⇶* t' ] -> *)
+(*       [Γ |- tQuote t ⤳* tQuote t' : tNat ]; *)
+(*     redtm_evalstep {Γ t u k n} : *)
+(*       [Γ |- t ≅ t : arr tNat tNat] -> *)
+(*       [Γ |- run : arr tNat (arr tNat tPNat)] -> *)
+(*       dnf t -> closed0 t -> *)
+(*       EvalStep Γ t u k n -> *)
+(*       [Γ |- tStep t (qNat u) ⤳* qNat k : tNat ]; *)
+(*     redtm_step {Γ t t' u u'} : *)
+(*       [Γ |- t ≅ t' : arr tNat tNat] -> *)
+(*       [Γ |- u ≅ u' : tNat] -> *)
+(*       [Γ |- run : arr tNat (arr tNat tPNat)] -> *)
+(*       [ t ⇶* t' ] -> *)
+(*       [ u ⇶* u' ] -> *)
+(*       dnf t' -> dnf u' -> *)
+(*       [Γ |- tStep t u ⤳* tStep t' u' : tNat ]; *)
+(*     redtm_evalreflect {Γ t t₀ u k n} : *)
+(*       [Γ |- t ≅ t₀ : arr tNat tNat] -> *)
+(*       [Γ |- run : arr tNat (arr tNat tPNat)] -> *)
+(*       dnf t₀ -> closed0 t₀ -> *)
+(*       EvalStep Γ t₀ u k n -> *)
+(*       [Γ |- tReflect t₀ (qNat u) ⤳* qEvalTm k n : tTotal t (qNat u) ]; *)
+(*     redtm_reflect {Γ t t' u u'} : *)
+(*       [Γ |- t ≅ t' : arr tNat tNat] -> *)
+(*       [Γ |- u ≅ u' : tNat] -> *)
+(*       [Γ |- run : arr tNat (arr tNat tPNat)] -> *)
+(*       [ t ⇶* t' ] -> *)
+(*       [ u ⇶* u' ] -> *)
+(*       dnf t' -> dnf u' -> *)
+(*       [Γ |- tReflect t u ⤳* tReflect t' u' : tTotal t u ]; *)
     redtm_conv {Γ t u A A'} :
       [Γ |- t ⤳* u : A] ->
       [Γ |- A ≅ A'] ->
@@ -2008,6 +2008,7 @@ Proof.
   + now apply convtm_evalBranchSucc.
 Qed.
 
+(*
 Lemma tTotal_cong {Γ t t' u u'} :
   [Γ |- tApp (tApp run (tQuote t)) u ≅ tApp (tApp run (tQuote t')) u' : arr tNat tNat] ->
   [Γ |- tStep t u ~ tStep t' u' : tNat] ->
@@ -2033,5 +2034,6 @@ intros; induction n; cbn.
     rewrite <- !(wk1_ren_on Γ (tId tNat tZero tZero)).
     apply ty_wk; [apply wfc_cons; gen_typing|tea].
 Qed.
+*)
 
 End EvalConsequences.
