theories/Syntax/NormalForms.v
@@ -51,9 +51,9 @@ with dne : term -> Set :=
   | dne_tFst {n} : dne n -> dne (tFst n)
   | dne_tSnd {n} : dne n -> dne (tSnd n)
   | dne_tIdElim {A x P hr y e} : dnf A -> dnf x -> dnf P -> dnf hr -> dnf y -> dne e -> dne (tIdElim A x P hr y e)
-  | dne_tQuote {t} : ~ closed0 t -> dnf t -> dne (tQuote t)
-  | dne_tStep {t u} : (~ is_closedn 0 t) + (~ is_closedn 0 u) -> dnf t -> dnf u -> dne (tStep t u)
-  | dne_tReflect {t u} : (~ is_closedn 0 t) + (~ is_closedn 0 u) -> dnf t -> dnf u -> dne (tReflect t u)
+  | dne_tDecide {A t u} : dnf A -> (~ is_closedn 0 t) + (~ is_closedn 0 u) -> dnf t -> dnf u -> dne (tDecide A t u)
+  | dne_tReflect {A t u e} : dnf A -> dnf t -> dnf u -> dne e -> dne (tReflect A t u e)
+  | dne_tReify {A t u e} : dnf A -> dnf t -> dnf u -> dne e -> dne (tReify A t u e)
 .
 
 Set Elimination Schemes.
@@ -90,9 +90,10 @@ with whne : term -> Type :=
   | whne_tFst {p} : whne p -> whne (tFst p)
   | whne_tSnd {p} : whne p -> whne (tSnd p)
   | whne_tIdElim {A x P hr y e} : whne e -> whne (tIdElim A x P hr y e)
-  | whne_tQuote {t} :  ~ closed0 t -> dnf t -> whne (tQuote t)
-  | whne_tStep {t u} : (~ is_closedn 0 t) + (~ is_closedn 0 u) -> dnf t -> dnf u -> whne (tStep t u)
-  | whne_tReflect {t u} : (~ is_closedn 0 t) + (~ is_closedn 0 u) -> dnf t -> dnf u -> whne (tReflect t u).
+  | whne_tDecide {A t u} : (~ is_closedn 0 t) + (~ is_closedn 0 u) -> dnf t -> dnf u -> whne (tDecide A t u)
+  | whne_tReflect {A t u e} : whne e -> whne (tReflect A t u e)
+  | whne_tReify {A t u e} : whne e -> whne (tReify A t u e)
+.
 
 #[global] Hint Constructors whne whnf : gen_typing.
 
@@ -146,7 +147,6 @@ Proof.
 unfold closed0; intros t Hc Ht; induction Ht; cbn in *; eauto.
 all: repeat match goal with H : _ |- _ => apply andb_prop in H; destruct H end; eauto.
 + destruct s; congruence.
-+ destruct s; congruence.
 Qed.
 
 Section RenDnf.
@@ -154,12 +154,7 @@ Section RenDnf.
 Lemma dnf_dne_ren : (forall t, dnf t -> forall ρ, dnf t⟨ρ⟩) × (forall t, dne t -> forall ρ, dne t⟨ρ⟩).
 Proof.
 apply dnf_dne_rect; cbn; intros; try now econstructor.
-+ constructor; [|now eauto].
-  intros Hc; now apply closed0_ren_rev in Hc.
-+ constructor; [|now eauto|now eauto].
-  destruct s; [left|right];
-  intros Hc; now apply closed0_ren_rev in Hc.
-+ constructor; [|now eauto|now eauto].
++ constructor; try now eauto.
   destruct s; [left|right];
   intros Hc; now apply closed0_ren_rev in Hc.
 Qed.
@@ -181,22 +176,12 @@ all: try now (
   match goal with H : dnf ?t |- _ => inversion H; subst; clear H end;
   match goal with H : dne ?t |- _ => inversion H; subst; clear H end;
   do 2 constructor; eauto; apply dne_dnf_whne; eauto using dnf_dne, dne_whne).
-+ inversion H; subst; inversion H2; subst.
-  do 2 constructor; [now eintros ?%closed0_ren|eauto].
-+ inversion H; subst.
-  constructor; [now eintros ?%closed0_ren|eauto].
-+ inversion H; subst; inversion H4; subst.
++ inversion H; subst; inversion H6; subst.
   do 2 constructor; eauto.
-  destruct H7; [left|right]; now eintros ?%closed0_ren.
+  destruct H11; [left|right]; now eintros ?%closed0_ren.
 + inversion H; subst.
   constructor; eauto.
-  destruct H6; [left|right]; now eintros ?%closed0_ren.
-+ inversion H; subst; inversion H4; subst.
-  do 2 constructor; eauto.
-  destruct H7; [left|right]; now eintros ?%closed0_ren.
-+ inversion H; subst.
-  constructor; eauto.
-  destruct H6; [left|right]; now eintros ?%closed0_ren.
+  destruct H9; [left|right]; now eintros ?%closed0_ren.
 Qed.
 
 Lemma dnf_ren_rev : forall t ρ, dnf t⟨ρ⟩ -> dnf t.
@@ -482,10 +467,6 @@ Section RenWhnf.
     split.
     - apply whne_ren_rev.
     - induction 1 ; cbn; try now econstructor.
-      + econstructor; [|now eapply dnf_ren].
-        intros Hc; now apply closed0_ren_rev in Hc.
-      + econstructor; try now eapply dnf_ren.
-        destruct s; [left|right]; intros Hc; now apply closed0_ren_rev in Hc.
       + econstructor; try now eapply dnf_ren.
         destruct s; [left|right]; intros Hc; now apply closed0_ren_rev in Hc.
   Qed.
@@ -599,9 +580,12 @@ Fixpoint is_nf ne t {struct t} := match t with
 | tSnd t => is_nf true t
 | tIdElim A x P hr y e =>
   is_nf false A && is_nf false x && is_nf false P && is_nf false hr && is_nf false y && is_nf true e
-| tQuote t => is_nf false t && negb (is_closedn 0 t)
-| tStep t u => is_nf false t && is_nf false u && (negb (is_closedn 0 t) || negb (is_closedn 0 u))
-| tReflect t u => is_nf false t && is_nf false u && (negb (is_closedn 0 t) || negb (is_closedn 0 u))
+| tDecide A t u =>
+  is_nf false A && is_nf false t && is_nf false u && (negb (is_closedn 0 t) || negb (is_closedn 0 u))
+| tReflect A t u e =>
+  is_nf false A && is_nf false t && is_nf false u && is_nf true e
+| tReify A t u e =>
+  is_nf false A && is_nf false t && is_nf false u && is_nf true e
 end.
 
 Definition is_dnf t := is_nf false t.
@@ -623,9 +607,9 @@ Fixpoint is_wnf ne t {struct t} := match t with
 | tFst t => is_wnf true t
 | tSnd t => is_wnf true t
 | tIdElim A x P hr y e => is_wnf true e
-| tQuote t => is_dnf t && negb (is_closedn 0 t)
-| tStep t u => is_dnf t && is_dnf u && (negb (is_closedn 0 t) || negb (is_closedn 0 u))
-| tReflect t u => is_dnf t && is_dnf u && (negb (is_closedn 0 t) || negb (is_closedn 0 u))
+| tDecide A t u => is_dnf t && is_dnf u && (negb (is_closedn 0 t) || negb (is_closedn 0 u))
+| tReflect A t u e => is_wnf true e
+| tReify A t u e => is_wnf true e
 end.
 
 Definition is_whnf t := is_wnf false t.
@@ -644,8 +628,6 @@ Proof.
 apply dnf_dne_rect; cbn; intros.
 all: repeat (apply andb_true_intro; split); eauto.
 + now apply is_nf_incl.
-+ now apply Bool.eq_true_not_negb.
-+ apply Bool.orb_true_intro; destruct s; [left|right]; now apply Bool.eq_true_not_negb.
 + apply Bool.orb_true_intro; destruct s; [left|right]; now apply Bool.eq_true_not_negb.
 Qed.
 
@@ -659,10 +641,6 @@ all: try discriminate.
 all: try match goal with |- dnf _ => constructor end.
 all: try match goal with |- dne _ => constructor end.
 all: eauto using dnf, dne.
-+ now eapply contraNnot.
-+ now eapply contraNnot.
-+ apply Bool.orb_true_elim in H0; destruct H0; [left|right]; now eapply contraNnot.
-+ apply Bool.orb_true_elim in H0; destruct H0; [left|right]; now eapply contraNnot.
 + apply Bool.orb_true_elim in H0; destruct H0; [left|right]; now eapply contraNnot.
 + apply Bool.orb_true_elim in H0; destruct H0; [left|right]; now eapply contraNnot.
 Qed.
@@ -692,11 +670,6 @@ Proof.
 induction 1; cbn.
 all: repeat (apply andb_true_intro; split); eauto using whne, whnf.
 + now eapply dnf_dne_is_nf.
-+ apply Bool.eq_true_not_negb; tea.
-+ now eapply dnf_dne_is_nf.
-+ now eapply dnf_dne_is_nf.
-+ apply Bool.orb_true_intro; destruct s; [left|right]; now apply Bool.eq_true_not_negb.
-+ now eapply dnf_dne_is_nf.
 + now eapply dnf_dne_is_nf.
 + apply Bool.orb_true_intro; destruct s; [left|right]; now apply Bool.eq_true_not_negb.
 Qed.
@@ -706,11 +679,6 @@ Proof.
 induction t; cbn; intros; try discriminate.
 all: repeat match goal with H : _ |- _ => apply andb_prop in H; destruct H end.
 all: eauto using whne, whnf.
-+ constructor.
-  - unfold closed0; destruct is_closedn; cbn in *; congruence.
-  - now apply is_nf_dnf_dne.
-+ constructor; try now apply is_nf_dnf_dne.
-  apply Bool.orb_true_elim in H0; destruct H0; [left|right]; now eapply contraNnot.
 + constructor; try now apply is_nf_dnf_dne.
   apply Bool.orb_true_elim in H0; destruct H0; [left|right]; now eapply contraNnot.
 Qed.
